src/Language/PlutusIR/Semantics/Static/Implementations/Named/ContextInvariance.v
@@ -1,0 +1,556 @@
+Require Import PlutusCert.Language.PlutusIR.
+Import NamedTerm.
+Require Import PlutusCert.Language.PlutusIR.Semantics.Static.
+Require Import PlutusCert.Language.PlutusIR.Semantics.Static.Implementations.Named.
+
+(* TODO: instead of using [term_vars_bound_by_bindings], use a separate inductive datatype that records boundness *)
+Require Import PlutusCert.Language.PlutusIR.Semantics.Dynamic.Substitution.
+
+Require Import Coq.Lists.List.
+
+
+Theorem context_invariance_T__has_kind : forall T ctx_T ctx_K K ctx_T',
+  (ctx_T, ctx_K) |-* T : K ->
+  (ctx_T', ctx_K) |-* T : K.
+Proof.
+  induction T.
+  - intros.
+    inversion H. subst.
+    apply K_Var.
+    assumption.
+  - intros.
+    inversion H. subst.
+    apply K_Fun. 
+    + eapply IHT1. eauto.
+    + eapply IHT2. eauto.
+  - intros.
+    inversion H. subst.
+    eapply K_IFix.
+    + eapply IHT2. eauto.
+    + eapply IHT1. eauto.
+  - intros. 
+    inversion H. subst.
+    apply K_Forall.
+    eapply IHT. eauto.
+  - intros.
+    inversion H. subst.
+    apply K_Builtin.
+  - intros.
+    inversion H. subst.
+    eapply K_Lam.
+    eapply IHT.
+    eauto.
+  - intros.
+    inversion H. subst.
+    eapply K_App.
+    + eapply IHT1. eauto.
+    + eapply IHT2. eauto.
+Qed.
+
+
+
+(** * Context invariance *)
+
+(** ** Type-level context invariance *)
+
+(** *** Free variables and closedness *)
+Inductive appears_free_in_Ty : tyname -> Ty -> Prop :=
+  | AFI_TyVar : forall X,
+      appears_free_in_Ty X (Ty_Var X)
+  | AFI_TyFun1 : forall X T1 T2,
+      appears_free_in_Ty X T1 ->
+      appears_free_in_Ty X (Ty_Fun T1 T2)
+  | AFI_TyFun2 : forall X T1 T2,
+      appears_free_in_Ty X T2 ->
+      appears_free_in_Ty X (Ty_Fun T1 T2)
+  | AFI_TyIFix1 : forall X F T,
+      appears_free_in_Ty X F ->
+      appears_free_in_Ty X (Ty_IFix F T)
+  | AFI_TyIFix2 : forall X F T,
+      appears_free_in_Ty X T ->
+      appears_free_in_Ty X (Ty_IFix F T)
+  | AFI_TyForall : forall X bX K T,
+      X <> bX ->
+      appears_free_in_Ty X T ->
+      appears_free_in_Ty X (Ty_Forall bX K T)
+  | AFI_TyLam : forall X bX K T,
+      X <> bX ->
+      appears_free_in_Ty X T ->
+      appears_free_in_Ty X (Ty_Lam bX K T)
+  | AFI_TyApp1 : forall X T1 T2,
+      appears_free_in_Ty X T1 ->
+      appears_free_in_Ty X (Ty_App T1 T2)
+  | AFI_TyApp2 : forall X T1 T2,
+      appears_free_in_Ty X T2 ->
+      appears_free_in_Ty X (Ty_App T1 T2)
+  .
+  
+#[export] Hint Constructors appears_free_in_Ty : core.
+
+Definition closed_typelevel  (T : Ty) :=
+  forall X, ~(appears_free_in_Ty X T).
+
+(** *** Context invariance (Lemma) *)
+Lemma context_invariance__typelevel : forall Gamma Gamma' T K,
+    Gamma |-* T : K ->
+    (forall X, appears_free_in_Ty X T -> lookupK Gamma X = lookupK Gamma' X) ->
+    Gamma' |-* T : K.
+Proof with auto.
+  intros Gamma Gamma' T K HK.
+  generalize dependent Gamma'.
+  induction HK; intros; try solve [econstructor; auto].
+  - apply K_Var.
+    rewrite <- H0...
+  - (* K_Forall *)
+    apply K_Forall.
+    apply IHHK.
+    intros.
+    destruct (X =? X0) eqn:Heqb.
+    + apply eqb_eq in Heqb.
+      subst.
+      rewrite lookupK_eq.
+      rewrite lookupK_eq.
+      reflexivity.
+    + apply eqb_neq in Heqb.
+      rewrite lookupK_neq...
+      rewrite lookupK_neq...
+  - (* K_Lam *)
+    apply K_Lam.
+    apply IHHK.
+    intros.
+    destruct (X =? X0) eqn:Heqb.
+    + apply eqb_eq in Heqb.
+      subst.
+      rewrite lookupK_eq.
+      rewrite lookupK_eq.
+      reflexivity.
+    + apply eqb_neq in Heqb.
+      rewrite lookupK_neq...
+      rewrite lookupK_neq...
+Qed.
+
+(** *** Free variables are in context (Lemma) *)
+
+Lemma free_in_context__typelevel : forall X T K Gamma,
+    appears_free_in_Ty X T ->
+    Gamma |-* T : K ->
+    exists K', lookupK Gamma X = Datatypes.Some K'.
+Proof with eauto.
+  intros X T K Gamma Hafi Htyp.
+  induction Htyp; inversion Hafi; subst...
+  - rewrite lookupK_neq in IHHtyp; auto.
+  - rewrite lookupK_neq in IHHtyp; auto.
+Qed.
+
+Corollary typable_empty__closed_typelevel : forall T K GammaT,
+    (GammaT, empty) |-* T : K ->
+    closed_typelevel T.
+Proof.
+  intros. unfold closed_typelevel. intros x H1.
+  destruct (free_in_context__typelevel _ _ _ _ H1 H) as [T' C].
+  discriminate C.
+Qed.
+
+(** ** Term-level context invariance *)
+
+(** *** Free variables and closedness *)
+Inductive appears_free_in : name -> Term -> Prop :=
+  | AFI_Let : forall x r bs t,
+      ~(In x (term_vars_bound_by_bindings bs)) ->
+      appears_free_in x t ->
+      appears_free_in x (Let r bs t)
+  | AFI_LetNonRec : forall x bs t,
+      appears_free_in_bindings_nonrec x bs ->
+      appears_free_in x (Let NonRec bs t)
+  | AFI_LetRec : forall x bs t,
+      ~(In x (term_vars_bound_by_bindings bs)) ->
+      appears_free_in_bindings_rec x bs ->
+      appears_free_in x (Let Rec bs t)
+  | AFI_Var : forall x,
+      appears_free_in x (Var x)
+  | AFI_TyAbs : forall x bX K t0,
+      appears_free_in x t0 ->
+      appears_free_in x (TyAbs bX K t0)
+  | AFI_LamAbs : forall x bx K t0,
+      x <> bx ->
+      appears_free_in x t0 ->
+      appears_free_in x (LamAbs bx K t0)
+  | AFI_Apply1 : forall x t1 t2,
+      appears_free_in x t1 ->
+      appears_free_in x (Apply t1 t2)
+  | AFI_Apply2 : forall x t1 t2,
+      appears_free_in x t2 ->
+      appears_free_in x (Apply t1 t2)
+  | AFI_TyInst : forall x t0 T,
+      appears_free_in x t0 ->
+      appears_free_in x (TyInst t0 T)
+  | AFI_IWrap : forall x F T t0,
+      appears_free_in x t0 ->
+      appears_free_in x (IWrap F T t0)
+  | AFI_Unwrap : forall x t0,
+      appears_free_in x t0 ->
+      appears_free_in x (Unwrap t0)
+
+with appears_free_in_bindings_nonrec : name -> list Binding -> Prop :=
+  | AFI_ConsB1_NonRec : forall x b bs,
+      appears_free_in_binding x b ->
+      appears_free_in_bindings_nonrec x (b :: bs)
+  | AFI_ConsB2_NonRec : forall x b bs,
+      ~(In x (term_vars_bound_by_binding b)) ->
+      appears_free_in_bindings_nonrec x bs ->
+      appears_free_in_bindings_nonrec x (b :: bs)
+
+with appears_free_in_bindings_rec : name -> list Binding -> Prop :=
+  | AFI_ConsB1_Rec : forall x b bs,
+      appears_free_in_binding x b ->
+      appears_free_in_bindings_rec x (b :: bs)
+  | AFI_ConsB2_Rec : forall x b bs,
+      appears_free_in_bindings_rec x bs ->
+      appears_free_in_bindings_rec x (b :: bs)
+
+with appears_free_in_binding : name -> Binding -> Prop :=
+  | AFI_TermBind : forall x s vd t0,
+      appears_free_in x t0 ->
+      appears_free_in_binding x (TermBind s vd t0)
+  .
+
+#[export] Hint Constructors 
+  appears_free_in 
+  appears_free_in_bindings_nonrec
+  appears_free_in_bindings_rec
+  appears_free_in_binding : core.
+
+Definition closed (t : Term) :=
+  forall x, ~(appears_free_in x t).
+
+(** ** Context invariance (Theorem) *)
+
+Definition P_has_type (Gamma : Context) (t : Term) (T : Ty) :=
+  forall Gamma',
+    (forall x, appears_free_in x t -> lookupT Gamma x = lookupT Gamma' x) ->
+    (forall X, lookupK Gamma X = lookupK Gamma' X) ->
+    Gamma' |-+ t : T.
+
+Definition P_constructor_well_formed (Gamma : Context) (c : constructor) :=
+  forall Gamma',
+    (forall X, lookupK Gamma X = lookupK Gamma' X) ->
+    Gamma' |-ok_c c.
+
+Definition P_bindings_well_formed_nonrec (Gamma : Context) (bs : list Binding) :=
+  forall Gamma',
+    (forall x, appears_free_in_bindings_nonrec x bs -> lookupT Gamma x = lookupT Gamma' x) ->
+    (forall X, lookupK Gamma X = lookupK Gamma' X) ->
+    Gamma' |-oks_nr bs.  
+
+Definition P_bindings_well_formed_rec (Gamma : Context) (bs : list Binding) :=
+  forall Gamma',
+    (forall x, appears_free_in_bindings_rec x bs -> lookupT Gamma x = lookupT Gamma' x) ->
+    (forall X, lookupK Gamma X = lookupK Gamma' X) ->
+    Gamma' |-oks_r bs.  
+
+Definition P_binding_well_formed (Gamma : Context) (b : Binding) :=
+  forall Gamma',
+    (forall x, appears_free_in_binding x b -> lookupT Gamma x = lookupT Gamma' x) ->
+    (forall X, lookupK Gamma X = lookupK Gamma' X) ->
+    Gamma' |-ok b.
+
+Axiom skip : forall P, P.
+
+Theorem context_invariance : 
+  (forall Gamma t T, Gamma |-+ t : T -> P_has_type Gamma t T) /\
+  (forall Gamma bs, Gamma |-oks_nr bs -> P_bindings_well_formed_nonrec Gamma bs) /\
+  (forall Gamma bs, Gamma |-oks_r bs -> P_bindings_well_formed_rec Gamma bs) /\
+  (forall Gamma b, Gamma |-ok b -> P_binding_well_formed Gamma b).
+Proof with eauto.
+  apply has_type__multind with
+    (P := P_has_type)
+    (P0 := P_constructor_well_formed)
+    (P1 := P_bindings_well_formed_nonrec)
+    (P2 := P_bindings_well_formed_rec)
+    (P3 := P_binding_well_formed).
+  - (* T_Let *)
+    intros. unfold P_has_type. intros.
+    subst.
+    eapply T_Let.
+    + reflexivity.
+    + apply H1.
+      * intros.
+        apply H4.
+        apply AFI_LetNonRec.
+        assumption.
+      * assumption.
+    + apply H3.
+      * intros.
+        apply lookupT_append_r.
+        apply H4.
+        apply AFI_Let.
+        -- apply skip. (* TODO *) 
+        -- assumption.
+      * intros.
+        apply lookupK_append_r.
+        apply H5.
+  - (* T_LetRec *)
+    intros. unfold P_has_type. intros.
+    subst.
+    eapply T_LetRec.
+    + reflexivity.
+    + apply H1.
+      * intros.
+        apply lookupT_append_r.
+        apply H4.
+        apply AFI_LetRec; auto.
+        apply skip. (* TODO *)
+      * intros.
+        apply lookupK_append_r.
+        apply H5.
+    + apply H3.
+      * intros.
+        apply lookupT_append_r.
+        apply H4.
+        apply AFI_Let.
+        -- apply skip. (* TODO *)
+        -- assumption.
+      * intros.
+        apply lookupK_append_r.
+        apply H5.
+  - (* T_Var *)
+    intros. unfold P_has_type. intros.
+    apply T_Var.
+    rewrite <- H0; auto.
+  - (* T_TyForall *)
+    intros. unfold P_has_type. intros.
+    apply T_TyAbs.
+    apply H0.
+    + intros x Hafi.
+      rewrite lookupT_extendK.
+      rewrite lookupT_extendK.
+      apply H1.
+      apply AFI_TyAbs.
+      assumption.
+    + intros Y.
+      destruct (X =? Y) eqn:Heqb.
+      * apply eqb_eq in Heqb.
+        subst.
+        rewrite lookupK_eq.
+        rewrite lookupK_eq.
+        reflexivity.
+      * apply eqb_neq in Heqb.
+        rewrite lookupK_neq; auto.
+        rewrite lookupK_neq; auto.
+  - (* T_LamAbs *)
+    intros. unfold P_has_type. intros.
+    apply T_LamAbs.
+    + apply H0.
+      * intros.
+        destruct (x =? x0) eqn:Heqb.
+        -- apply eqb_eq in Heqb.
+          subst.
+          rewrite lookupT_eq.
+          rewrite lookupT_eq.
+          reflexivity.
+        -- apply eqb_neq in Heqb.
+          rewrite lookupT_neq; auto.
+          rewrite lookupT_neq; auto.
+      * intros.
+        -- rewrite lookupK_extendT.
+           rewrite lookupK_extendT.
+           apply H3.
+    + apply context_invariance__typelevel with ctx.
+      * assumption.
+      * intros.
+        apply H3.
+  - (* T_Apply *)
+    intros. unfold P_has_type. intros.
+    apply T_Apply with T1.
+    + apply H0.
+      * intros.
+        apply H3.
+        apply AFI_Apply1.
+        assumption.
+      * intros.
+        apply H4.
+    + apply H2.
+      * intros.
+        apply H3.
+        apply AFI_Apply2.
+        assumption.
+      * intros.
+        apply H4.
+  - (* T_Constant *)
+    intros. unfold P_has_type. intros.
+    apply T_Constant.
+  - (* T_Builtin *)
+    intros. unfold P_has_type. intros.
+    apply T_Builtin.
+  - (* T_TyInst *)
+    intros. unfold P_has_type. intros.
+    apply T_TyInst with T1 X K2.
+    + apply H0.
+      * intros.
+        apply H3.
+        apply AFI_TyInst.
+        assumption.
+      * intros.
+        apply H4.
+    + apply context_invariance__typelevel with ctx.
+      * assumption.
+      * intros.
+        apply H4.
+    + assumption.
+  - (* T_Error *)
+    intros. unfold P_has_type. intros.
+    apply T_Error.
+    apply context_invariance__typelevel with ctx.
+    + assumption.
+    + intros.
+      apply H1.
+  - (* T_IWrap *)
+    intros. unfold P_has_type. intros.
+    apply T_IWrap with K S.
+    + assumption.
+    + apply H1.
+      * intros.
+        apply H4.
+        apply AFI_IWrap.
+        assumption.
+      * intros.
+        apply H5.
+    + apply context_invariance__typelevel with ctx.
+      * assumption.
+      * intros.
+        apply H5.
+    + apply context_invariance__typelevel with ctx.
+      * assumption.
+      * intros.
+        apply H5.
+  - (* T_Unwrap *)
+    intros. unfold P_has_type. intros.
+    apply T_Unwrap with F K T.
+    + apply H0.
+      * intros.
+        apply H3.
+        apply AFI_Unwrap.
+        assumption.
+      * intros.
+        apply H4.
+    + apply context_invariance__typelevel with ctx.
+      * assumption.
+      * intros.
+        apply H4.
+    + assumption.
+  
+  - (* W_Con *)
+    intros. unfold P_constructor_well_formed. intros.
+    constructor.
+    intros.
+    destruct Gamma'.
+    destruct ctx.
+    eapply context_invariance_T__has_kind.
+    eapply context_invariance__typelevel.
+    + apply H.
+      assumption.
+    + intros.
+      apply H0.
+  
+  - (* W_NilB_NonRec *)
+    intros. unfold P_bindings_well_formed_nonrec. intros.
+    constructor.
+  - (* W_ConsB_NonRec *)
+    intros. unfold P_bindings_well_formed_nonrec. intros.
+    apply W_ConsB_NonRec.
+    + apply H0.
+      intros.
+      apply H3.
+      apply AFI_ConsB1_NonRec.
+      * assumption.
+      * assumption.
+    + apply H2.
+      intros.
+      apply lookupT_append_r.
+      apply H3.
+      apply AFI_ConsB2_NonRec.
+      * unfold P_binding_well_formed in H0.
+        unfold P_bindings_well_formed_nonrec in H2. apply skip. (* TODO *) 
+      * assumption.
+      * intros.
+        apply lookupK_append_r.
+        apply H4.
+  
+  - (* W_NilB_Rec *)
+    intros. unfold P_bindings_well_formed_rec. intros.
+    constructor.
+  - (* W_ConsB_Rec *)
+    intros. unfold P_bindings_well_formed_rec. intros.
+    apply W_ConsB_Rec.
+    + apply H0.
+      * intros.
+        apply H3.
+        apply AFI_ConsB1_Rec.
+        assumption.
+      * assumption.
+    + apply H2.
+      * intros.
+        apply H3.
+        apply AFI_ConsB2_Rec.
+        assumption.
+      * assumption.
+  
+  - (* W_Term *)
+    intros. unfold P_binding_well_formed. intros.
+    apply W_Term.
+    + apply context_invariance__typelevel with ctx.
+      * assumption.
+      * intros.
+        apply H3.
+    + apply H1.
+      * intros.
+        apply H2.
+        apply AFI_TermBind.
+        assumption.
+      * intros.
+        apply H3.
+  - (* W_Type *)
+    intros. unfold P_binding_well_formed. intros.
+    apply W_Type.
+    apply context_invariance__typelevel with ctx.
+    * assumption.
+    * intros.
+      apply H1.
+  - (* W_Data *)
+    intros. unfold P_binding_well_formed. intros.
+    subst.
+    eapply W_Data.
+    + reflexivity.
+    + intros.
+      apply H1.
+      * assumption. 
+      * intros.
+        apply lookupK_append_r.
+        apply H3.
+Qed.
+
+    
+
+Lemma free_in_context : forall x t T Gamma,
+    appears_free_in x t ->
+    Gamma |-+ t : T ->
+    exists T', lookupT Gamma x = Datatypes.Some T'.
+Proof. Admitted.
+
+Corollary typable_empty__closed : forall t T,
+    emptyContext |-+ t : T ->
+    closed t.
+Proof.
+  intros. unfold closed. intros x H1.
+  destruct (free_in_context _ _ _ _ H1 H) as [T' C].
+  discriminate C.
+Qed.
+
+Corollary typable_emptyT__closed : forall ctxK t T,
+    (empty, ctxK) |-+ t : T ->
+    closed t.
+Proof.
+  intros. unfold closed. intros x H1.
+  destruct (free_in_context _ _ _ _ H1 H) as [T' C].
+  discriminate C.
+Qed.
